ifc-machine/pico/tmu/cmach/ConcreteMachineSmallStep.v
@@ -12,43 +12,63 @@ Local Open Scope Z_scope.
 
 (** Reflexive transitive closure. *)
 (* to be moved in Utils *)
-Inductive star (S: Type) (Rstep: S -> S -> Prop): S -> S -> Prop :=
+
+Definition op_cons (E: Type) (oe: option E) (l: list E) :=
+  match oe with 
+      | Some e => e::l
+      | None => l
+  end.
+
+Inductive star (S E: Type) (Rstep: S -> option E -> S -> Prop): S -> list E -> S -> Prop :=
   | star_refl: forall s,
-      star Rstep s s
-  | star_step: forall s1 s2 s3,
-      Rstep s1 s2 -> star Rstep s2 s3 -> 
-      star Rstep s1 s3.
+      star Rstep s nil s
+  | star_step: forall s1 s2 s3 e t t',
+      Rstep s1 e s2 -> star Rstep s2 t s3 -> 
+      t' = (op_cons e t) ->
+      star Rstep s1 t' s3.
 Hint Constructors star.
 
-Lemma star_right : forall S (Rstep: S -> S -> Prop) s1 s2, 
-                     star Rstep s1 s2 -> 
-                     forall s3, 
-                       Rstep s2 s3 -> star Rstep s1 s3.
+Lemma op_cons_app : forall E (e: option E) t t', (op_cons e t)++t' = op_cons e (t++t').
+Proof. intros. destruct e; reflexivity. Qed.  
+
+Lemma star_right : forall S E (Rstep: S -> option E -> S -> Prop) s1 s2 t, 
+                     star Rstep s1 t s2 -> 
+                     forall s3 e t', 
+                       Rstep s2 e s3 -> 
+                       t' = (t++(op_cons e nil)) ->
+                       star Rstep s1 t' s3.
 Proof.
   induction 1; intros.
   eapply star_step; eauto.
-  eauto.
+  exploit IHstar; eauto. intros.
+  inv H3. rewrite op_cons_app; eauto. 
 Qed.
 
-Inductive plus (S: Type) (Rstep: S -> S -> Prop): S -> S -> Prop :=
-  | plus_step: forall s s',
-      Rstep s s' ->
-      plus Rstep s s'
-  | plus_trans: forall s1 s2 s3,
-      Rstep s1 s2 -> plus Rstep s2 s3 -> 
-      plus Rstep s1 s3.
+Inductive plus (S E: Type) (Rstep: S -> option E -> S -> Prop): S -> list E -> S -> Prop :=
+  | plus_step: forall s t s' e,
+      Rstep s e s' ->
+      t = (op_cons e nil) ->
+      plus Rstep s t s'
+  | plus_trans: forall s1 s2 s3 e t t',
+      Rstep s1 e s2 -> plus Rstep s2 t s3 -> 
+      t' = (op_cons e t) ->
+      plus Rstep s1 t' s3.
 
 Hint Constructors star.
 Hint Constructors plus.
 
-Lemma plus_right : forall S (Rstep: S -> S -> Prop) s1 s2, 
-                     plus Rstep s1 s2 -> 
-                     forall s3, 
-                       Rstep s2 s3 -> plus Rstep s1 s3.
+Lemma plus_right : forall E S (Rstep: S -> option E -> S -> Prop) s1 s2 t, 
+                     plus Rstep s1 t s2 -> 
+                     forall s3 e t',
+                       t' = (t++(op_cons e nil)) ->
+                       Rstep s2 e s3 -> plus Rstep s1 t' s3.
 Proof.
   induction 1; intros.
+  inv H1.
+  rewrite op_cons_app. simpl.
   eapply plus_trans; eauto.
-  eauto.
+  exploit IHplus; eauto.
+  inv H2. rewrite op_cons_app.  eauto.
 Qed.
 
 Section CMach.
@@ -61,81 +81,81 @@ Notation fh_ret := (fun pc pcl => (CRet (pc,pcl) false false)).
 (** Concrete machine transition relation.
     Each instructions has 3 semantic rules: (user mode - succ) (user mode - faulting) (kernel mode) *)
 
-Inductive cstep : CS -> CS -> Prop := 
+Inductive cstep : CS -> option CEvent -> CS -> Prop := 
 | cstep_nop : forall c m fh i s pcv pcl rl rpcl,
     forall (INST: i @ pcv # Noop)
            (CHIT: cache_hit c (opCodeToZ OpNoop) (__,__,__) pcl)
            (CREAD: cache_hit_read c rl rpcl),
     cstep (CState c m fh i s (pcv,pcl) false)
-          (CState c m fh i s (pcv+1,rpcl) false)
+          None (CState c m fh i s (pcv+1,rpcl) false)
 
 | cstep_nop_f : forall c c' m fh i s pcv pcl,
    forall (INST: i @ pcv # Noop)
           (CMISS: ~ cache_hit c (opCodeToZ OpNoop) (__,__,__) pcl)
           (CUPD: c' = build_cache (opCodeToZ OpNoop) (__,__,__)  pcl),
     cstep (CState c m fh i s (pcv,pcl) false) 
-          (CState c' m fh i ((fh_ret pcv pcl)::s) fh_start true)
+          None (CState c' m fh i ((fh_ret pcv pcl)::s) fh_start true)
 
 | cstep_nop_p : forall c m fh i s pcv pcl,
     fh @ pcv # Noop ->
-    cstep (CState c m fh i s (pcv,pcl) true) (CState c m fh i s (pcv+1,pcl) true)
+    cstep (CState c m fh i s (pcv,pcl) true) None (CState c m fh i s (pcv+1,pcl) true)
 
 | cstep_add: forall c fh m i s rpcl pcv pcl rl x1v x1l x2v x2l,
    forall(INST: i @ pcv # Add)
          (CHIT: cache_hit c (opCodeToZ OpAdd) (x1l, x2l, __) pcl)
          (CREAD: cache_hit_read c rl rpcl),
      cstep (CState c m fh i ((x1v,x1l):::(x2v,x2l):::s) (pcv,pcl)    false)  
-           (CState c m fh i          ((x1v+x2v,rl):::s) (pcv+1,rpcl) false)
+           None (CState c m fh i          ((x1v+x2v,rl):::s) (pcv+1,rpcl) false)
 
 | cstep_add_f: forall c c' fh m i s pcv pcl x1v x1l x2v x2l,
    forall(INST: i @ pcv # Add)
          (CMISS: ~ cache_hit c (opCodeToZ OpAdd) (x1l, x2l, __) pcl)
          (CUPD: c' = build_cache (opCodeToZ OpAdd) (x1l,x2l,__)  pcl),
      cstep (CState c  m fh i ((x1v,x1l):::(x2v,x2l):::s) (pcv,pcl)    false)  
-           (CState c' m fh i ((fh_ret pcv pcl)::(x1v,x1l):::(x2v,x2l):::s) fh_start true)
+           None (CState c' m fh i ((fh_ret pcv pcl)::(x1v,x1l):::(x2v,x2l):::s) fh_start true)
 
 | cstep_add_p: forall c m fh i s pcv pcl x1v x1l x2v x2l, 
     fh @ pcv # Add ->
     cstep (CState c m fh i ((x1v,x1l):::(x2v,x2l):::s) (pcv,pcl) true)  
-          (CState c m fh i ((x1v+x2v,handlerTag):::s) (pcv+1,pcl) true)
+          None (CState c m fh i ((x1v+x2v,handlerTag):::s) (pcv+1,pcl) true)
 
 | cstep_sub: forall c fh m i s rpcl pcv  pcl rl x1v x1l x2v x2l,
    forall(INST: i @ pcv # Sub)
          (CHIT: cache_hit c (opCodeToZ OpSub) (x1l, x2l, __) pcl)
          (CREAD: cache_hit_read c rl rpcl),
      cstep (CState c m fh i ((x1v,x1l):::(x2v,x2l):::s) (pcv,pcl)    false)  
-           (CState c m fh i          ((x1v-x2v,rl):::s) (pcv+1,rpcl) false)
+           None (CState c m fh i          ((x1v-x2v,rl):::s) (pcv+1,rpcl) false)
 
 | cstep_sub_f: forall c c' fh m i s pcv pcl x1v x1l x2v x2l,
    forall(INST: i @ pcv # Sub)
          (CMISS: ~ cache_hit c (opCodeToZ OpSub) (x1l, x2l, __) pcl)
          (CUPD: c' = build_cache (opCodeToZ OpSub) (x1l,x2l,__)  pcl),
      cstep (CState c  m fh i ((x1v,x1l):::(x2v,x2l):::s) (pcv,pcl)    false)  
-           (CState c' m fh i ((fh_ret pcv pcl)::(x1v,x1l):::(x2v,x2l):::s) fh_start true)
+           None (CState c' m fh i ((fh_ret pcv pcl)::(x1v,x1l):::(x2v,x2l):::s) fh_start true)
 
 | cstep_sub_p: forall c m fh i s pcv pcl x1v x1l x2v x2l, 
     fh @ pcv # Sub ->
     cstep (CState c m fh i ((x1v,x1l):::(x2v,x2l):::s) (pcv,pcl) true) 
-          (CState c m fh i ((x1v-x2v,handlerTag):::s) (pcv+1,pcl) true)
+          None (CState c m fh i ((x1v-x2v,handlerTag):::s) (pcv+1,pcl) true)
 
 | cstep_push: forall c fh m i s rpcl pcv pcl rl cv,
    forall(INST: i @ pcv # Push cv)
          (CHIT: cache_hit c (opCodeToZ OpPush) (__ , __, __) pcl)
          (CREAD: cache_hit_read c rl rpcl),
      cstep (CState c m fh i s (pcv,pcl)   false)
-           (CState c m fh i ((cv,rl):::s) (pcv+1,rpcl) false)
+           None (CState c m fh i ((cv,rl):::s) (pcv+1,rpcl) false)
 
 | cstep_push_f: forall c c' fh m i s pcv pcl cv,
    forall(INST : i @ pcv # Push cv)
          (CMISS: ~ cache_hit c (opCodeToZ OpPush) (__,__,__) pcl)
          (CUPD : c' = build_cache (opCodeToZ OpPush) (__,__,__) pcl),
      cstep (CState c  m fh i s (pcv,pcl) false)  
-           (CState c' m fh i ((fh_ret pcv pcl)::s) fh_start true)
+           None (CState c' m fh i ((fh_ret pcv pcl)::s) fh_start true)
 
 | cstep_push_p: forall c m fh i s pcv pcl cv, 
     fh @ pcv # Push cv ->
     cstep (CState c m fh i s (pcv,pcl) true) 
-          (CState c m fh i ((cv,handlerTag):::s) (pcv+1,pcl) true)
+          None (CState c m fh i ((cv,handlerTag):::s) (pcv+1,pcl) true)
 
 | cstep_load: forall c fh m i s rpcl pcv pcl rl addrv addrl xv xl,
    forall(INST: i @ pcv # Load)
@@ -143,7 +163,7 @@ Inductive cstep : CS -> CS -> Prop :=
          (CREAD: cache_hit_read c rl rpcl)
          (MREAD: read_m addrv m = Some (xv,xl)),
      cstep (CState c m fh i ((addrv,addrl):::s) (pcv,pcl)   false)
-           (CState c m fh i ((xv,rl):::s) (pcv+1,rpcl) false)
+           None (CState c m fh i ((xv,rl):::s) (pcv+1,rpcl) false)
 
 | cstep_load_f: forall c c' fh m i s pcv pcl addrv addrl xv xl,
    forall(INST: i @ pcv # Load)
@@ -151,13 +171,13 @@ Inductive cstep : CS -> CS -> Prop :=
          (MREAD: read_m addrv m = Some (xv,xl))
          (CUPD : c' = build_cache (opCodeToZ OpLoad) (addrl,xl,__) pcl),
      cstep (CState c  m fh i ((addrv,addrl):::s) (pcv,pcl)   false)
-           (CState c' m fh i ((fh_ret pcv pcl)::(addrv,addrl):::s) fh_start true)
+           None (CState c' m fh i ((fh_ret pcv pcl)::(addrv,addrl):::s) fh_start true)
 
 | cstep_load_p: forall c m fh i s pcv pcl addrv addrl xv xl,
     fh @ pcv # Load ->
     read_m addrv c = Some (xv,xl) ->
     cstep (CState c m fh i ((addrv,addrl):::s) (pcv,pcl) true) 
-          (CState c m fh i ((xv,handlerTag):::s) (pcv+1,pcl) true)
+          None (CState c m fh i ((xv,handlerTag):::s) (pcv+1,pcl) true)
 
 | cstep_store: forall c fh m m' i s rpcl pcv pcl rl addrv addrl xv xl mv ml,
    forall(INST: i @ pcv # Store)
@@ -166,7 +186,7 @@ Inductive cstep : CS -> CS -> Prop :=
          (MREAD: read_m addrv m = Some (mv,ml))
          (MUPDT: upd_m addrv (xv,rl) m = Some m'),
      cstep (CState c m fh i ((addrv,addrl):::(xv,xl):::s) (pcv,pcl)   false)
-           (CState c m' fh i s (pcv+1,rpcl) false)
+           None (CState c m' fh i s (pcv+1,rpcl) false)
 
 | cstep_store_f: forall c c' fh m i s pcv pcl addrv addrl xv xl mv ml,
    forall(INST: i @ pcv # Store)
@@ -174,51 +194,51 @@ Inductive cstep : CS -> CS -> Prop :=
          (MREAD: read_m addrv m = Some (mv,ml))
          (CUPD : c' = build_cache (opCodeToZ OpStore) (addrl,xl,ml) pcl),
      cstep (CState c  m fh i ((addrv,addrl):::(xv,xl):::s) (pcv,pcl)   false)
-           (CState c' m fh i ((fh_ret pcv pcl)::(addrv,addrl):::(xv,xl):::s) fh_start true)
+           None (CState c' m fh i ((fh_ret pcv pcl)::(addrv,addrl):::(xv,xl):::s) fh_start true)
 
 | cstep_store_p: forall c m fh i s pcv pcl c' addrv addrl x, 
     fh @ pcv # Store ->
     upd_m addrv x c = Some c' ->
     cstep (CState c m fh i ((addrv,addrl)::: x :::s) (pcv,pcl) true)
-          (CState c' m fh i s (pcv+1,pcl) true)
+          None (CState c' m fh i s (pcv+1,pcl) true)
 
 | cstep_jump: forall c fh m i s rpcl pcv pcl rl cv cl,
    forall(INST: i @ pcv # Jump)
          (CHIT: cache_hit c (opCodeToZ OpJump) (cl, __, __) pcl)
          (CREAD: cache_hit_read c rl rpcl),
      cstep (CState c m fh i ((cv,cl):::s) (pcv,pcl)   false)
-           (CState c m fh i s (cv,rpcl) false)
+           None (CState c m fh i s (cv,rpcl) false)
 
 | cstep_jump_f: forall c c' fh m i s pcv pcl cv cl,
    forall(INST: i @ pcv # Jump)
          (CMISS: ~ cache_hit c (opCodeToZ OpJump) (cl,__,__) pcl)
          (CUPD : c' = build_cache (opCodeToZ OpJump) (cl,__,__) pcl),
      cstep (CState c  m fh i ((cv,cl):::s) (pcv,pcl)   false)
-           (CState c' m fh i ((fh_ret pcv pcl)::(cv,cl):::s) fh_start true)
+           None (CState c' m fh i ((fh_ret pcv pcl)::(cv,cl):::s) fh_start true)
 
 | cstep_jump_p: forall c m fh i s pcv pcl pcj pcjl,
     fh @ pcv # Jump ->
     cstep (CState c m fh i ((pcj,pcjl):::s) (pcv,pcl) true) 
-          (CState c m fh i s (pcj,pcjl) true)
+          None (CState c m fh i s (pcj,pcjl) true)
 
 | cstep_bnz: forall c fh m i s rpcl pcv pcl rl cv cl offv,
    forall(INST: i @ pcv # BranchNZ offv)
          (CHIT: cache_hit c (opCodeToZ OpBranchNZ) (cl, __, __) pcl)
          (CREAD: cache_hit_read c rl rpcl),
      cstep (CState c m fh i ((cv,cl):::s) (pcv,pcl)   false)
-           (CState c m fh i s (if cv =? 0 then pcv+1 else pcv+offv, rpcl) false)
+           None (CState c m fh i s (if cv =? 0 then pcv+1 else pcv+offv, rpcl) false)
 
 | cstep_bnz_f: forall c c' fh m i s pcv pcl cv cl offv,
    forall(INST: i @ pcv # BranchNZ offv)
          (CMISS: ~ cache_hit c (opCodeToZ OpBranchNZ) (cl,__,__) pcl)
          (CUPD : c' = build_cache (opCodeToZ OpBranchNZ) (cl,__,__) pcl),
      cstep (CState c  m fh i ((cv,cl):::s) (pcv,pcl)   false)
-           (CState c' m fh i ((fh_ret pcv pcl)::(cv,cl):::s) fh_start true)
+           None (CState c' m fh i ((fh_ret pcv pcl)::(cv,cl):::s) fh_start true)
 
 | cstep_branchnz_p: forall c m fh i s pcv pcl offv av al,
     fh @ pcv # BranchNZ offv -> 
     cstep (CState c m fh i ((av,al):::s) (pcv,pcl) true) 
-          (CState c m fh i s (if av =? 0 then pcv+1 else pcv+offv, handlerTag) true)
+          None (CState c m fh i s (if av =? 0 then pcv+1 else pcv+offv, handlerTag) true)
 
 | cstep_call: forall c fh m i s rpcl pcv pcl rl pcc pccl a r args,
    forall(INST: i @ pcv # Call a r)
@@ -227,7 +247,7 @@ Inductive cstep : CS -> CS -> Prop :=
          (CHIT: cache_hit c (opCodeToZ OpCall) (pccl, __, __) pcl)
          (CREAD: cache_hit_read c rl rpcl),
      cstep (CState c m fh i ((pcc,pccl):::args++s) (pcv,pcl)   false)
-           (CState c m fh i (args++(((CRet (pcv+1, rl)) r false)::s)) (pcc,rpcl) false)
+           None (CState c m fh i (args++(((CRet (pcv+1, rl)) r false)::s)) (pcc,rpcl) false)
 
 | cstep_call_f: forall c c' fh m i s pcv pcl pcc pccl a r args,
    forall(INST: i @ pcv # Call a r)
@@ -236,13 +256,13 @@ Inductive cstep : CS -> CS -> Prop :=
          (CMISS: ~ cache_hit c (opCodeToZ OpCall) (pccl, __, __) pcl)
          (CUPD : c' = build_cache (opCodeToZ OpCall) (pccl,__,__) pcl),
      cstep (CState c  m fh i ((pcc,pccl):::args++s) (pcv,pcl)   false)
-           (CState c' m fh i ((fh_ret pcv pcl)::(pcc,pccl):::args++s) fh_start true)
+           None (CState c' m fh i ((fh_ret pcv pcl)::(pcc,pccl):::args++s) fh_start true)
 
 | cstep_call_p: forall c m fh i s pcv pcl a r args pcc pccl,
     fh @ pcv # Call a r -> 
     length args = a -> (forall a, In a args -> exists d, a = CData d) ->
     cstep (CState c m fh i ((pcc,pccl):::args++s) (pcv,pcl) true) 
-          (CState c m fh i (args++(CRet (pcv+1, pcl) r true)::s) (pcc, pccl) true)
+          None (CState c m fh i (args++(CRet (pcv+1, pcl) r true)::s) (pcc, pccl) true)
 
 | cstep_ret: forall c fh m i s s' pcv pcl rl rpcl pcret pcretl,
    forall(INST: i @ pcv # Ret)
@@ -251,7 +271,7 @@ Inductive cstep : CS -> CS -> Prop :=
                 (*DD: should only return to user mode *)
          (CREAD: cache_hit_read c rl rpcl),
      cstep (CState c m fh i s  (pcv,pcl) false)
-           (CState c m fh i s' (pcret, rpcl) false)
+           None (CState c m fh i s' (pcret, rpcl) false)
 
 | cstep_ret_f: forall c c' fh m i s' s pcv pcl pcret pcretl,
    forall(INST: i @ pcv # Ret)
@@ -259,13 +279,13 @@ Inductive cstep : CS -> CS -> Prop :=
          (POP:  c_pop_to_return s ((CRet (pcret,pcretl) false false)::s')) (*DD: same thing *)
          (CUPD : c' = build_cache (opCodeToZ OpRet) (pcretl,__,__) pcl),
      cstep (CState c m fh i s  (pcv,pcl) false)
-           (CState c' m fh i ((fh_ret pcv pcl)::s) fh_start true)
+           None (CState c' m fh i ((fh_ret pcv pcl)::s) fh_start true)
 
 | cstep_ret_p: forall c m fh i s pcv pcl  pcret pcretl s' pret, 
     fh @ pcv # Ret -> (* can either return to user/priv mode *)
     c_pop_to_return s ((CRet (pcret,pcretl) false pret)::s') ->
     cstep (CState c m fh i s  (pcv,pcl) true) 
-          (CState c m fh i s' (pcret,pcretl) pret)
+          None (CState c m fh i s' (pcret,pcretl) pret)
 
 | cstep_vret: forall c fh m i s s' pcv pcl rl rpcl resv resl pcret pcretl,
    forall(INST: i @ pcv # VRet)
@@ -274,7 +294,7 @@ Inductive cstep : CS -> CS -> Prop :=
                 (*DD: should only return to user mode *)
          (CREAD: cache_hit_read c rl rpcl),
      cstep (CState c m fh i ((resv,resl):::s)  (pcv,pcl) false)
-           (CState c m fh i ((resv,rl):::s') (pcret,rpcl) false)
+           None (CState c m fh i ((resv,rl):::s') (pcret,rpcl) false)
 
 | cstep_vret_f: forall c c' fh m i s' s pcv pcl resv resl pcret pcretl,
    forall(INST: i @ pcv # VRet)
@@ -282,13 +302,27 @@ Inductive cstep : CS -> CS -> Prop :=
          (POP:  c_pop_to_return s ((CRet (pcret,pcretl) true false)::s')) (*DD: same thing *)
          (CUPD : c' = build_cache (opCodeToZ OpVRet) (resl,pcretl,__) pcl),
      cstep (CState c m fh i ((resv,resl):::s)  (pcv,pcl) false)
-           (CState c' m fh i ((fh_ret pcv pcl)::(resv,resl):::s) fh_start true)
+           None (CState c' m fh i ((fh_ret pcv pcl)::(resv,resl):::s) fh_start true)
 
 | cstep_vret_p: forall c m fh i s pcv pcl s' pcret pcretl resv resl, 
     fh @ pcv # VRet -> (* cannot vreturn to user mode *)
     c_pop_to_return s ((CRet (pcret,pcretl) true true)::s') ->
     cstep (CState c m fh i ((resv,resl):::s) (pcv,pcl) true) 
-          (CState c m fh i ((resv,resl):::s') (pcret, pcretl) true).
+          None (CState c m fh i ((resv,resl):::s') (pcret, pcretl) true)
+
+| cstep_out: forall c fh m i s rpcl pcv pcl rl cv cl,
+   forall(INST: i @ pcv # Output)
+         (CHIT: cache_hit c (opCodeToZ OpOutput) (cl, __, __) pcl)
+         (CREAD: cache_hit_read c rl rpcl),
+     cstep (CState c m fh i ((cv,cl):::s) (pcv,pcl)   false)
+           (Some (CEInt (cv,rl))) (CState c m fh i s (pcv+1,rpcl) false)
+
+| cstep_out_f: forall c c' fh m i s pcv pcl cv cl,
+   forall(INST: i @ pcv # Output)
+         (CMISS: ~ cache_hit c (opCodeToZ OpOutput) (cl,__,__) pcl)
+         (CUPD : c' = build_cache (opCodeToZ OpOutput) (cl,__,__) pcl),
+     cstep (CState c  m fh i ((cv,cl):::s) (pcv,pcl)   false)
+           None (CState c' m fh i ((fh_ret pcv pcl)::(cv,cl):::s) fh_start true).
 
 (* Success is reaching a Halt state in non-privileged mode and valid address. *)
 Definition c_success (cs : CS) : Prop :=
@@ -297,39 +331,40 @@ Definition c_success (cs : CS) : Prop :=
   | _ => False
   end.
 
-Inductive runsToEscape : CS -> CS -> Prop :=
+Inductive runsToEscape : CS -> list CEvent -> CS -> Prop :=
 | rte_success: (* executing until a return to user mode *)
-    forall cs cs',
+    forall cs cs' t,
     forall (PRIV:  priv cs = true)
-           (STAR:  star cstep cs cs')
+           (STAR:  star cstep cs t cs')
            (UPRIV: priv cs' = false), 
-      runsToEscape cs cs'
+      runsToEscape cs t cs'
 | rte_fail : (* executing the tmu until it fails at a neg. pc in priv mode *)
-    forall cs cs',
+    forall cs cs' t,
     forall (PRIV: priv cs = true)
-           (STAR: star cstep cs cs')
+           (STAR: star cstep cs t cs')
            (PRIV: priv cs' = true)
            (FAIL: fst (pc cs') < 0), 
-      runsToEscape cs cs'
+      runsToEscape cs t cs'
 | rte_upriv: (* in unpriv. mode, it already escaped *) 
     forall cs,
     forall (UPRIV: priv cs = false),
-      runsToEscape cs cs.
+      runsToEscape cs nil cs.
 
-Lemma step_star_plus (S: Type): 
-  forall (Rstep: S -> S -> Prop) (s2 s3: S), 
-    star Rstep s2 s3 ->
-    forall s1, 
-      Rstep s1 s2 ->
-      plus Rstep s1 s3.
+Lemma step_star_plus (S E: Type): 
+  forall (Rstep: S -> option E -> S -> Prop) (s2 s3: S) t, 
+    star Rstep s2 t s3 ->
+    forall s1 e t', 
+      Rstep s1 e s2 ->
+      t' = (op_cons e t) ->
+      plus Rstep s1 t' s3.
 Proof.
   induction 1; intros; eauto.
 Qed.
 
-Lemma runsToEscape_star: forall s1 s2, 
- runsToEscape s1 s2 ->
+Lemma runsToEscape_star: forall s1 s2 t, 
+ runsToEscape s1 t s2 ->
  s1 <> s2 ->
- plus cstep s1 s2.
+ plus cstep s1 t s2.
 Proof.
   induction 1 ; intros;
   try ( inv STAR; [ congruence | eapply step_star_plus; eauto]).
