ifc-machine/pico/tmu/cmach/FaultRoutine.v
@@ -79,7 +79,7 @@ Definition genCheckOp (op:OpCode): code :=
 Definition fetch_rule_impl_type: Type := forall (opcode:OpCode),  {n:nat & AllowModify n}.
 Variable fetch_rule_impl: fetch_rule_impl_type.
 Definition opcodes := 
-  [OpNoop; OpAdd; OpSub; OpPush; OpLoad; OpStore; OpJump; OpBranchNZ; OpCall; OpRet; OpVRet].
+  [OpNoop; OpAdd; OpSub; OpPush; OpLoad; OpStore; OpJump; OpBranchNZ; OpCall; OpRet; OpVRet; OpOutput].
 Definition genApplyRule' op := genApplyRule (projT2 (fetch_rule_impl op)).
 (* Fault handler that puts results on stack. *)
 Definition genFaultHandlerStack: code :=
@@ -1035,7 +1035,7 @@ Conjecture handler_correct :
     cache_hit c (opCodeToZ opcode) (labsToZs vls) (labToZ pcl) ->
     exists c' st pc priv, 
       runsToEscape (CState c m fhdl imem (CRet retaddr false false::s) (0,handlerTag) true)
-                   (CState c' m fhdl imem st pc priv) /\ 
+                   nil (CState c' m fhdl imem st pc priv) /\ 
       match apply_rule (projT2 am) vls pcl with
         | Some (olr,lpc) => handler_final_mem_matches' olr lpc c c' 
                      /\ pc = retaddr
@@ -1060,7 +1060,7 @@ Theorem handler_correct_succeed :
          (RULE: apply_rule (projT2 (get_rule opcode)) vls pcl = Some (olr,lpc)),
     exists c',
     runsToEscape (CState c m handler i (CRet raddr false false::s) (0,handlerTag) true)
-                 (CState c' m handler i s raddr false) /\
+                 nil (CState c' m handler i s raddr false) /\
     handler_final_mem_matches' olr lpc c c'.
 Proof.
   intros.
@@ -1097,7 +1097,7 @@ Conjecture handler_correct_fail :
          (RULE: apply_rule (projT2 (get_rule opcode)) vls pcl = None),
     exists st,
     runsToEscape (CState c m handler i (CRet raddr false false::s) (0,handlerTag) true)
-                 (CState c m handler i st (-1,handlerTag) true).
+                 nil (CState c m handler i st (-1,handlerTag) true).
 
 (*  We also have the following: 
     - the handler code terminates DONE
